doc/developer/semantics/Mz.lean
@@ -2,4 +2,5 @@ import Mz.Datum
 import Mz.Expr
 import Mz.Eval
 import Mz.Boolean
+import Mz.MightError
 import Mz.Laws
